Distributivity lore

DeBruijnSSA/BinSyntax/Rewrite/Region/Compose/Distrib.lean
@@ -89,7 +89,25 @@ theorem Eqv.distl_inv_distl {A B C : Ty α} {Γ : Ctx α ε} {L : LCtx α}
   ;; distl = nil := by
   rw [distl_eq_ret, distl_inv_eq_ret, <-ret_of_seq, Term.Eqv.distl_inv_distl_pure]; rfl
 
-def Eqv.rtimes_sum_seq_distl_inv {A B C : Ty α} {Γ : Ctx α ε} {L : LCtx α}
+theorem Eqv.distl_seq_injective {A B C : Ty α} {Γ : Ctx α ε}
+  {r s : Eqv φ (⟨A.prod (B.coprod C), ⊥⟩::Γ) (D::L)} (h : distl ;; r = distl ;; s)
+  : r = s := by
+  rw [<-nil_seq r, <-nil_seq s, <-distl_inv_distl, seq_assoc, h, seq_assoc]
+
+theorem Eqv.rtimes_inj_l_seq_distl_inv {A B C : Ty α} {Γ : Ctx α ε} {L : LCtx α}
+  : A ⋊ inj_l ;; distl_inv (φ := φ) (A := A) (B := B) (C := C) (Γ := Γ) (L := L) = inj_l := by
+  sorry
+
+theorem Eqv.rtimes_inj_r_seq_distl_inv {A B C : Ty α} {Γ : Ctx α ε} {L : LCtx α}
+  : A ⋊ inj_r ;; distl_inv (φ := φ) (A := A) (B := B) (C := C) (Γ := Γ) (L := L) = inj_r := by
+  sorry
+
+theorem Eqv.rtimes_sum_seq_distl_inv {A B C : Ty α} {Γ : Ctx α ε} {L : LCtx α}
   {l : Eqv φ ((A, ⊥)::Γ) (A'::L)} {r : Eqv φ ((B, ⊥)::Γ) (B'::L)}
   : C ⋊ (sum l r) ;; distl_inv = distl_inv ;; sum (C ⋊ l) (C ⋊ r)
-  := sorry
+  := by
+  apply distl_seq_injective
+  rw [<-seq_assoc, <-seq_assoc, distl_distl_inv, nil_seq, distl, coprod_seq, coprod_seq, sum]
+  congr 1
+  · rw [rtimes_rtimes, inj_l_coprod, <-rtimes_rtimes, seq_assoc, rtimes_inj_l_seq_distl_inv]
+  · rw [rtimes_rtimes, inj_r_coprod, <-rtimes_rtimes, seq_assoc, rtimes_inj_r_seq_distl_inv]
